pulse/share/steel/examples/pulse/dice/engine/EngineCore.fsti
@@ -10,15 +10,15 @@ val l0_is_authentic (repr:engine_record_repr) : prop
 val cdi_functional_correctness (c0:Seq.seq U8.t) (repr:engine_record_repr) : prop 
 
 val engine_main (cdi:cdi_t) (uds:A.larray U8.t (SZ.v uds_len)) (record:engine_record_t)
-                (#p:perm)
                 (#c0:Ghost.erased (elseq U8.t dice_digest_len))
                 (#repr:Ghost.erased engine_record_repr)
-  : stt dice_return_code (A.pts_to uds p uds_bytes **
-                          A.pts_to cdi full_perm c0 **
-                          engine_record_perm record repr)
+                (#uds_perm #p:perm)
+  : stt dice_return_code (engine_record_perm record repr p **
+                          A.pts_to uds uds_perm uds_bytes **
+                          A.pts_to cdi full_perm c0)
                          (fun r -> 
-                            engine_record_perm record repr **
-                            A.pts_to uds p uds_bytes **
+                            engine_record_perm record repr p **
+                            A.pts_to uds uds_perm uds_bytes **
                             exists_ (fun (c1:elseq U8.t dice_digest_len) ->
                                       A.pts_to cdi full_perm c1 **
                                       pure (A.is_full_array cdi
